Bank_SN.v
@@ -10,7 +10,7 @@ Section Bank_SN.
   Definition bank_sn_base_params    := base_params.
   Definition bank_sn_multi_params   := multi_params.
   Definition bank_sn_failure_params := bank_failure_params.
-  
+
   Definition bank_sn_network :=
-  @network bank_sn_base_params bank_sn_multi_params.
+    @network bank_sn_base_params bank_sn_multi_params.
 End Bank_SN.
