Bank_SN_Proofs.v
@@ -1,24 +1,33 @@
-Require Import Bank.
-Require Import Bank_Proofs.
-Require Import Bank_SN.
-Require Import Verdi.SeqNum.
-Require Import Verdi.Verdi.
-Require Import Verdi.SeqNumCorrect.
+Require Import
+  Bank
+  Bank_SN
+  Bank_Proofs.
+
+From Verdi Require Import
+  Verdi
+  SeqNum
+  SeqNumCorrect.
+
+From InfSeqExt Require Import
+  infseq
+  exteq.
 
 Set Bullet Behavior "Strict Subproofs".
 
 Section Bank_SN_Proofs.
-  (*What about traces??*)
-  Theorem transformed_correctness :
+
+  (* What about traces?? *)
+  Theorem transformed_min_value_invariant :
     forall (net : bank_sn_network) tr,
       step_dup_star (params := bank_sn_multi_params) step_async_init net tr ->
       min_value_invariant_net (revertNetwork net).
   Proof using.
-  intros. 
-  pose proof @true_in_reachable_transform _ bank_multi_params 
-             (fun net : network => min_value_invariant_net net)
-             true_in_reachable_min_value.
-  unfold true_in_reachable in *.
-  apply H0. unfold reachable. eauto.
+    intros.
+    pose proof @true_in_reachable_transform _ bank_multi_params 
+               (fun net : network => min_value_invariant_net net)
+               true_in_reachable_min_value.
+    unfold true_in_reachable in *.
+    apply H0. unfold reachable. eauto.
   Qed.
+
 End Bank_SN_Proofs.
